src/AsyncFSDiskSecVictim.v
@@ -1,0 +1,244 @@
+Require Import Mem Word.
+Require Import Omega.
+Require Import Bool.
+Require Import Pred.
+Require Import GenSepN.
+Require Import ListPred.
+Require Import List ListUtils.
+Require Import Bytes.
+Require Import Rec.
+Require Import Arith.
+Require Import FSLayout.
+Require Import Errno.
+Require Import Lia.
+Require Import FunctionalExtensionality.
+Require Import FMapAVL.
+Require Import FMapFacts.
+Require Import Prog ProgLoop ProgList.
+Require Import ProgAuto.
+Require Import DestructPair.
+Import ListNotations.
+
+Set Implicit Arguments.
+
+Parameter can_access_dec: forall pr t, {can_access pr t}+{~can_access pr t}.
+
+
+Definition equivalent_for tag (d1 d2: rawdisk) :=
+  forall a,
+    (d1 a = None /\ d2 a = None) \/
+    (exists vs1 vs2,
+       d1 a = Some vs1 /\ d2 a = Some vs2 /\
+       Forall2 (fun tb1 tb2 => fst tb1 = fst tb2) (vsmerge vs1) (vsmerge vs2) /\
+       Forall2 (fun tb1 tb2 => fst tb1 = tag -> snd tb1 = snd tb2) (vsmerge vs1) (vsmerge vs2)).
+
+
+Definition blockmem_equivalent_for tag (bm1 bm2: block_mem) :=
+  forall a,
+    (bm1 a = None /\ bm2 a = None) \/
+    (exists v1 v2,
+       bm1 a = Some v1 /\ bm2 a = Some v2 /\
+       fst v1 = fst v2 /\
+       (fst v1 = tag -> snd v1 = snd v2)).
+
+
+Definition same_except tag (d1 d2: rawdisk) :=
+  forall a,
+    (d1 a = None /\ d2 a = None) \/
+    (exists vs1 vs2,
+       d1 a = Some vs1 /\ d2 a = Some vs2 /\
+       Forall2 (fun tb1 tb2 => fst tb1 = fst tb2) (vsmerge vs1) (vsmerge vs2) /\
+       Forall2 (fun tb1 tb2 => fst tb1 <> tag -> snd tb1 = snd tb2) (vsmerge vs1) (vsmerge vs2)).
+
+Definition blockmem_same_except tag (bm1 bm2: block_mem) :=
+  forall a,
+    (bm1 a = None /\ bm2 a = None) \/
+    (exists v1 v2,
+       bm1 a = Some v1 /\ bm2 a = Some v2 /\
+       fst v1 = fst v2 /\
+       (fst v1 <> tag -> snd v1 = snd v2)).
+
+Lemma exec_blockmem_subset_upd:
+        forall T (p: prog T) pr d bm hm h v d1 bm1 hm1 r1 tr,
+          exec pr d (upd bm h v) hm p (Finished d1 bm1 hm1 r1) tr ->
+          exists bm1', bm1 = upd bm1' h v /\ (bm h = None -> bm1' h = None). 
+  Proof.
+    induction p; intros; inv_exec_perm;
+    try solve [ eexists; intuition eauto ];
+    try solve [ destruct (handle_eq_dec h r1); subst;
+    [ rewrite upd_eq in *; eauto; congruence
+    | rewrite upd_comm; eauto; eexists;
+      intuition eauto; rewrite upd_ne; eauto] ].
+    specialize IHp with (1:=H0); cleanup.
+    specialize H with (1:=H1); cleanup.
+    eexists; intuition eauto.
+  Qed.
+
+  Fixpoint only_public_operations tr :=
+    match tr with
+    | nil => True
+    | op::tr' =>
+      match op with
+      | Uns t => t = Public
+      | Sea t => t = Public
+      end /\ only_public_operations tr'
+    end.
+
+  Lemma only_public_operations_app:
+    forall tr1 tr2,
+      only_public_operations (tr1++tr2) ->
+      only_public_operations tr1 /\ only_public_operations tr2.
+  Proof.
+    induction tr1; simpl; intuition;
+    specialize IHtr1 with (1:= H1); cleanup; auto.
+  Qed.
+
+  Lemma blockmem_same_except_upd_same:
+    forall t bm bm' h b b0,
+      blockmem_same_except t bm bm' ->
+      blockmem_same_except t (upd bm h (t, b)) (upd bm' h (t, b0)).
+  Proof.
+    unfold blockmem_same_except; intros.
+    destruct (handle_eq_dec h a); subst.
+    repeat rewrite upd_eq; eauto.
+    right.
+    simpl in *; do 2 eexists; intuition eauto.
+    simpl in *; intuition.
+    repeat rewrite upd_ne in *; eauto.
+  Qed.
+
+  Lemma blockmem_same_except_upd_eq:
+    forall t bm bm' h v,
+      blockmem_same_except t bm bm' ->
+      blockmem_same_except t (upd bm h v) (upd bm' h v).
+  Proof.
+    unfold blockmem_same_except; intros.
+    destruct (handle_eq_dec h a); subst.
+    repeat rewrite upd_eq; eauto.
+    right.
+    simpl in *; do 2 eexists; intuition eauto.
+    repeat rewrite upd_ne in *; eauto.
+  Qed.
+
+
+  Lemma same_except_upd_same:
+    forall t d d' n b b0 b1 b2 t2 l l0,
+      same_except t d d' ->
+      Forall2 (fun tb1 tb2 => fst tb1 <> t -> snd tb1 = snd tb2)
+              (vsmerge (t2, b1, l)) (vsmerge (t2, b2, l0)) ->
+      Forall2 (fun tb1 tb2 => fst tb1 = fst tb2) l l0 ->
+      same_except t (upd d n (t, b, vsmerge (t2, b1, l)))
+                  (upd d' n (t, b0, vsmerge (t2, b2, l0))).
+  Proof.
+    unfold same_except; intros.
+    destruct (addr_eq_dec n a); subst.
+    repeat rewrite upd_eq; eauto.
+    right.
+    simpl in *; do 2 eexists; intuition eauto.
+    unfold vsmerge in *; simpl in *; intuition.
+    unfold vsmerge in *; simpl in *; intuition.
+    repeat rewrite upd_ne in *; eauto. 
+  Qed.
+
+
+  Lemma same_except_upd_eq:
+    forall t d d' n b b1 b2 t1 t2 l l0,
+      same_except t d d' ->
+      Forall2 (fun tb1 tb2 => fst tb1 <> t -> snd tb1 = snd tb2)
+              (vsmerge (t2, b1, l)) (vsmerge (t2, b2, l0)) ->
+      Forall2 (fun tb1 tb2 => fst tb1 = fst tb2) l l0 ->
+      same_except t (upd d n (t1, b, vsmerge (t2, b1, l)))
+                  (upd d' n (t1, b, vsmerge (t2, b2, l0))).
+  Proof.
+    unfold same_except; intros.
+    destruct (addr_eq_dec n a); subst.
+    repeat rewrite upd_eq; eauto.
+    right.
+    simpl in *; do 2 eexists; intuition eauto.
+    unfold vsmerge in *; simpl in *; intuition.
+    unfold vsmerge in *; simpl in *; intuition.
+    repeat rewrite upd_ne in *; eauto. 
+  Qed.
+
+  Lemma same_except_sync_mem:
+    forall t d d',
+      same_except t d d' ->
+      same_except t (sync_mem d) (sync_mem d').
+  Proof.
+    unfold sync_mem, same_except; intros.
+    specialize (H a); split_ors; cleanup; eauto.
+    destruct x, x0; simpl in *.
+    right.
+    simpl in *; do 2 eexists; intuition eauto.
+    unfold vsmerge in *; simpl in *; intuition.
+    inversion H1; eauto.
+    unfold vsmerge in *; simpl in *; intuition.
+    inversion H2; eauto.
+  Qed.
+  
+  Lemma exec_same_except_finished:
+  forall T (p: prog T) pr d d' bm bm' hm t d1 bm1 hm1 r1 tr,
+    exec pr d bm hm p (Finished d1 bm1 hm1 r1) tr ->
+    same_except t d d' ->
+    blockmem_same_except t bm bm' ->
+    only_public_operations tr ->
+    t <> Public ->
+    exists d2 bm2,
+      exec pr d' bm' hm p (Finished d2 bm2 hm1 r1) tr /\
+      same_except t d1 d2 /\
+      blockmem_same_except t bm1 bm2.
+  Proof.
+    induction p; intros; inv_exec_perm;
+    try solve [do 2 eexists; split; try econstructor; eauto].
+    {
+      specialize (H1 r1) as Hx; split_ors; cleanup; try congruence.
+      specialize (H0 n) as Hx; split_ors; cleanup; try congruence.
+      destruct x0.
+      do 2 eexists; split; try econstructor; eauto.
+      destruct tb, t0; unfold vsmerge in *;  simpl in *.
+      inversion H7; subst; simpl in *; clear H7; subst.
+      inversion H8; subst; simpl in *; clear H8; subst.
+      destruct (tag_dec t0 t); subst.
+      apply blockmem_same_except_upd_same; auto.
+      rewrite H10; eauto.
+      apply blockmem_same_except_upd_eq; auto.
+    }
+    {
+      destruct tb; cleanup.
+      specialize (H1 h) as Hx; split_ors; cleanup; try congruence.
+      destruct x0; simpl in *; cleanup.
+      specialize (H0 n) as Hx; split_ors; cleanup; try congruence.
+      destruct x, x0, t0, t2; simpl in *.
+      do 2 eexists; split; try econstructor; eauto.
+      inversion H7; subst; simpl in *; clear H7; subst.
+      destruct (tag_dec t1 t); subst.
+      eapply same_except_upd_same; eauto.
+      rewrite H6; eauto.
+      eapply same_except_upd_eq; eauto.
+    }
+    {
+      specialize (H1 r1) as Hx; split_ors; cleanup; try congruence.
+      do 2 eexists; split; try econstructor; eauto.
+      apply blockmem_same_except_upd_eq; auto.
+    }
+    {
+      destruct tb; cleanup.
+      specialize (H1 h) as Hx; split_ors; cleanup; try congruence.
+      do 2 eexists; split; try econstructor; eauto.
+      destruct x0; cleanup.
+      simpl fst in *; subst.
+      eapply ExecUnseal.
+      simpl in *; cleanup.
+      rewrite H6; intuition.
+    }
+    {
+      do 2 eexists; split; try econstructor; eauto.
+      apply same_except_sync_mem; auto.
+    }
+    {
+      apply only_public_operations_app in H3; cleanup.
+      specialize IHp with (1:=H0)(2:=H1)(3:=H2)(4:=H6)(5:=H4); cleanup.
+      specialize H with (1:=H5)(2:=H8)(3:=H9)(4:=H3)(5:=H4); cleanup.
+      do 2 eexists; split; try econstructor; eauto.
+    }
+  Qed.
