src/AsyncFSProg.v
@@ -1,0 +1,301 @@
+Require Import Word.
+Require Import Omega.
+Require Import Bool.
+Require Import Pred.
+Require Import DirCache.
+Require Import GenSepN.
+Require Import ListPred.
+Require Import Inode.
+Require Import List ListUtils.
+Require Import Bytes.
+Require Import DirTree.
+Require Import Rec.
+Require Import Arith.
+Require Import FSLayout.
+Require Import Errno.
+Require Import SuperBlock.
+Require Import Lia.
+Require Import FunctionalExtensionality.
+Require Import BFile.
+Require Import DirTreeDef.
+Require Import DirTreeRep.
+Require Import DirTreePred.
+Require Import DirTreeInodes.
+Require Import DirTreeSafe.
+Require Import DirTreeNames.
+Require Import AsyncFS.
+
+Set Implicit Arguments.
+Import DirTree.
+Import DIRTREE.
+Import AFS.
+Import ListNotations.
+
+Notation MSLL := BFILE.MSLL.
+Notation MSAllocC := BFILE.MSAllocC.
+Notation MSIAllocC := BFILE.MSIAllocC.
+Notation MSICache := BFILE.MSICache.
+Notation MSAlloc := BFILE.MSAlloc.
+Notation MSDBlocks := BFILE.MSDBlocks.
+
+
+(** Safety **)
+
+(** 
+(** this axioms may simplify tree equivalence after execution proofs *)
+Axiom one_tag_per_user:
+  forall pr t t',
+    t <> Public ->
+    t' <> Public ->
+    can_access pr t ->
+    can_access pr t' ->
+    t = t'.
+
+Axiom one_user_per_tag:
+  forall pr pr' t,
+    t <> Public ->
+    can_access pr t ->
+    can_access pr' t ->
+    pr = pr'.
+ *)
+
+Inductive fbasic : Type -> Type :=
+| file_get_attr_f :
+    INODE.IRec.Cache.key ->
+    fbasic (Rec.data (Rec.field_type
+            (Rec.FE [("owner", Rec.WordF 8);
+                     ("unused", Rec.WordF 16)]
+                    "attr" INODE.attrtype)))
+
+| file_set_attr_f :
+    INODE.IRec.Cache.key ->
+    INODE.iattrin ->
+    fbasic (res unit)
+
+| file_get_sz_f :
+    INODE.IRec.Cache.key ->
+    fbasic (word 64)
+
+| file_set_sz_f :
+    INODE.IRec.Cache.key ->
+    word 64 ->
+    fbasic (res unit)
+                         
+| read_fblock_f :
+    INODE.IRec.Cache.key ->
+    addr ->
+    fbasic (res block)
+
+| update_fblock_d_f :
+    INODE.IRec.Cache.key ->
+    addr ->
+    block ->
+    fbasic (res unit)
+           
+| file_truncate_f :
+    INODE.IRec.Cache.key ->
+    addr ->
+    fbasic (res unit)
+
+| file_sync_f :
+    INODE.IRec.Cache.key ->
+    fbasic (res unit)
+
+| readdir_f :
+    INODE.IRec.Cache.key ->
+    fbasic (list (String.string * (addr * bool)))
+
+| mkdir_f :
+    BFcache.key ->
+    Dcache.key ->
+    fbasic (res addr)
+
+| mksock_f :
+    BFcache.key ->
+    Dcache.key ->
+    tag ->
+    fbasic (res INODE.IRec.Cache.key)
+
+| create_f :
+    BFcache.key ->
+    Dcache.key ->
+    tag ->
+    fbasic (res addr)
+           
+| delete_f :
+    BFcache.key ->
+    Dcache.key ->
+    fbasic (res unit)
+
+| lookup_f :
+    addr ->
+    list String.string ->
+    fbasic (res (BFcache.key * bool))
+           
+| rename_f :
+    addr ->
+    list String.string ->
+    Dcache.key ->
+    list String.string ->
+    Dcache.key ->
+    fbasic (res unit)
+
+| tree_sync_f :
+    fbasic (res unit)
+
+| tree_sync_noop_f :
+    fbasic (res unit).
+
+Inductive fprog : Type -> Type :=
+| FBasic : forall T, fbasic T -> fprog T
+| FBind: forall T T', fbasic T  -> (T -> fprog T') -> fprog T'.
+
+Inductive exec_fbasic:
+  forall T, perm -> tagged_disk ->
+       block_mem -> hashmap -> fs_xparams -> BFILE.memstate ->
+       fbasic T ->  @result T -> BFILE.memstate -> trace -> Prop :=
+| FExecRead    :
+    forall pr d bm hm tr' fsxp inum off (ams ams': BFILE.memstate)
+      (r: res block) d' bm' hm',
+      exec pr d bm hm (read_fblock fsxp inum off ams)
+           (Finished d' bm' hm' ^(ams', r)) tr' ->
+      exec_fbasic pr d bm hm fsxp ams (read_fblock_f inum off)
+                  (Finished d' bm' hm' r) ams' tr'
+                  
+| FExecSetAttr    :
+    forall pr d bm hm tr' fsxp inum (ams ams': BFILE.memstate)
+      attr (r: res unit) d' bm' hm',
+      exec pr d bm hm (file_set_attr fsxp inum attr ams)
+           (Finished d' bm' hm' ^(ams', r)) tr' ->
+      exec_fbasic pr d bm hm fsxp ams (file_set_attr_f inum attr)
+                  (Finished d' bm' hm' r) ams' tr'
+
+| FExecGetAttr    :
+    forall pr d bm hm tr' fsxp inum (ams ams': BFILE.memstate)
+      r d' bm' hm',
+      exec pr d bm hm (file_get_attr fsxp inum ams)
+           (Finished d' bm' hm' ^(ams', r)) tr' ->
+      exec_fbasic pr d bm hm fsxp ams (file_get_attr_f inum)
+                  (Finished d' bm' hm' r) ams' tr'
+
+| FExecSetSz    :
+    forall pr d bm hm tr' fsxp inum (ams ams': BFILE.memstate)
+      sz (r: res unit) d' bm' hm',
+      exec pr d bm hm (file_set_sz fsxp inum sz ams)
+           (Finished d' bm' hm' ^(ams', r)) tr' ->
+      exec_fbasic pr d bm hm fsxp ams (file_set_sz_f inum sz)
+                  (Finished d' bm' hm' r) ams' tr'
+
+| FExecGetSz    :
+    forall pr d bm hm tr' fsxp inum (ams ams': BFILE.memstate)
+      r d' bm' hm',
+      exec pr d bm hm (file_get_sz fsxp inum ams)
+           (Finished d' bm' hm' ^(ams', r)) tr' ->
+      exec_fbasic pr d bm hm fsxp ams (file_get_sz_f inum)
+            (Finished d' bm' hm' r) ams' tr'
+                   
+| FExecWrite   :
+    forall pr d bm hm d' bm' hm' tr' fsxp
+      inum off v (ams ams': BFILE.memstate) (ok: res unit),
+      exec pr d bm hm (update_fblock_d fsxp inum off v ams)
+           (Finished d' bm' hm' ^(ams', ok)) tr' ->
+      exec_fbasic pr d bm hm fsxp ams (update_fblock_d_f inum off v)
+                  (Finished d' bm' hm' ok) ams' tr'
+
+| FExecTruncate    :
+    forall pr d bm hm tr' fsxp inum (ams ams': BFILE.memstate)
+      sz (r: res unit) d' bm' hm',
+      exec pr d bm hm (file_truncate fsxp inum sz ams)
+           (Finished d' bm' hm' ^(ams', r)) tr' ->
+      exec_fbasic pr d bm hm fsxp ams (file_truncate_f inum sz)
+                  (Finished d' bm' hm' r) ams' tr'
+
+| FExecFileSync    :
+    forall pr d bm hm tr' fsxp inum (ams ams': BFILE.memstate)
+      (r: res unit) d' bm' hm',
+      exec pr d bm hm (file_sync fsxp inum ams)
+           (Finished d' bm' hm' ^(ams', r)) tr' ->
+      exec_fbasic pr d bm hm fsxp ams (file_sync_f inum)
+                  (Finished d' bm' hm' r) ams' tr'
+
+| FExecReaddir    :
+    forall pr d bm hm tr' fsxp inum (ams ams': BFILE.memstate)
+      (r: list (String.string * (addr * bool))) d' bm' hm',
+      exec pr d bm hm (readdir fsxp inum ams)
+           (Finished d' bm' hm' ^(ams', r)) tr' ->
+      exec_fbasic pr d bm hm fsxp ams (readdir_f inum)
+                  (Finished d' bm' hm' r) ams' tr'
+
+| FExecCreate    :
+    forall pr d bm hm tr' fsxp dnum (ams ams': BFILE.memstate)
+      (r: res addr) name tag d' bm' hm',
+      exec pr d bm hm (create fsxp dnum name tag ams)
+           (Finished d' bm' hm' ^(ams', r)) tr' ->
+      exec_fbasic pr d bm hm fsxp ams (create_f dnum name tag)
+                  (Finished d' bm' hm' r) ams' tr'
+
+| FExecDelete    :
+    forall pr d bm hm tr' fsxp dnum (ams ams': BFILE.memstate)
+      (r: res unit) name d' bm' hm',
+      exec pr d bm hm (delete fsxp dnum name ams)
+           (Finished d' bm' hm' ^(ams', r)) tr' ->
+      exec_fbasic pr d bm hm fsxp ams (delete_f dnum name)
+                  (Finished d' bm' hm' r) ams' tr'
+
+| FExecLookup    :
+    forall pr d bm hm tr' fsxp dnum (ams ams': BFILE.memstate)
+      (r: res (BFcache.key * bool)) fnlist d' bm' hm',
+      exec pr d bm hm (lookup fsxp dnum fnlist ams)
+           (Finished d' bm' hm' ^(ams', r)) tr' ->
+      exec_fbasic pr d bm hm fsxp ams (lookup_f dnum fnlist)
+                  (Finished d' bm' hm' r) ams' tr'
+
+| FExecRename    :
+    forall pr d bm hm tr' fsxp dnum (ams ams': BFILE.memstate)
+      (r: res unit) srcpath srcname dstpath dstname d' bm' hm',
+      exec pr d bm hm (rename fsxp dnum srcpath srcname dstpath dstname ams)
+           (Finished d' bm' hm' ^(ams', r)) tr' ->
+      exec_fbasic pr d bm hm fsxp ams (rename_f dnum srcpath srcname dstpath dstname)
+                  (Finished d' bm' hm' r) ams' tr'
+
+| FExecTreeSync    :
+    forall pr d bm hm tr' fsxp (ams ams': BFILE.memstate)
+      (r: res unit) d' bm' hm',
+      exec pr d bm hm (tree_sync fsxp ams)
+           (Finished d' bm' hm' ^(ams', r)) tr' ->
+      exec_fbasic pr d bm hm fsxp ams (tree_sync_f)
+                  (Finished d' bm' hm' r) ams' tr'
+
+| FExecTreeSyncNoop    :
+    forall pr d bm hm tr' fsxp (ams ams': BFILE.memstate)
+      (r: res unit) d' bm' hm',
+      exec pr d bm hm (tree_sync_noop fsxp ams)
+           (Finished d' bm' hm' ^(ams', r)) tr' ->
+      exec_fbasic pr d bm hm fsxp ams (tree_sync_noop_f)
+                  (Finished d' bm' hm' r) ams' tr'.
+
+
+Inductive fexec:
+  forall T, perm -> tagged_disk ->
+       block_mem -> hashmap -> fs_xparams -> BFILE.memstate ->
+       fprog T ->  @result T -> BFILE.memstate -> trace -> Prop :=
+| FExecBasic    :
+    forall T (p :fbasic T) pr fsxp d bm hm tr' (ams ams': BFILE.memstate)
+     out,
+      exec_fbasic pr d bm hm fsxp ams p out ams' tr' ->
+      fexec pr d bm hm fsxp ams (FBasic p) out ams' tr'
+                   
+| FExecBind :
+    forall T T' pr (p1 : fbasic T) (p2: T -> fprog T') fsxp d bm hm d'
+      bm' hm' v r tr' tr'' ams ams' ams'',
+               exec_fbasic pr d bm hm fsxp ams p1 (Finished d' bm' hm' v) ams' tr' ->
+               fexec pr d' bm' hm' fsxp ams' (p2 v) r ams'' tr'' ->
+               fexec pr d bm hm fsxp ams (FBind p1 p2) r ams'' (tr''++tr')
+
+| FCrashBind : forall T T' pr (p1 : fbasic T) (p2: T -> fprog T') fsxp d d' bm bm' hm hm' tr' ams ams',
+                exec_fbasic pr d bm hm fsxp ams p1 (Crashed d' bm' hm') ams' tr' ->
+                fexec pr d bm hm fsxp ams (FBind p1 p2) (Crashed d' bm' hm') ams' tr'
+
+| FFailedBind : forall T T' pr (p1 : fbasic T) (p2: T -> fprog T') fsxp d d' bm bm' hm hm' tr' ams ams',
+                exec_fbasic pr d bm hm fsxp ams p1 (Failed d' bm' hm') ams' tr' ->
+                fexec pr d bm hm fsxp ams (FBind p1 p2) (Failed d' bm' hm') ams' tr'.
