src/TwoExecExample.v
@@ -1,0 +1,686 @@
+Fixpoint filter tag tree:=
+  match tree with
+  | TreeFile inum f =>
+    if tag_dec tag (DFOwner f) then
+      TreeFile inum f
+    else
+      TreeFile inum (mk_dirfile nil INODE.iattr0 (DFOwner f))
+  | TreeDir inum ents =>
+    TreeDir inum (map (fun st => (fst st, filter tag (snd st))) ents)
+  end.
+
+Definition equivalent_for tag tree1 tree2:=
+  filter tag tree1 = filter tag tree2.
+
+Definition public_equivalent tree1 tree2:=
+  equivalent_for Public tree1 tree2.
+
+Definition same_except tag tree1 tree2:=
+  forall tag', tag' <> tag -> equivalent_for tag' tree1 tree2.
+
+Definition same_except_nonpublic tag tree1 tree2:=
+  forall tag', tag'<> Public -> tag' <> tag -> equivalent_for tag' tree1 tree2.
+
+Definition fbasic_to_prog {T} mscs (fp: fbasic T): prog (BFILE.memstate * (T * unit)) :=
+  match fp with
+  | FRead fsxp inum off => read_fblock fsxp inum off mscs
+  | FWrite fsxp inum off v => update_fblock_d fsxp inum off v mscs
+  end.
+
+Fixpoint fprog_to_prog {T} mscs (fp: fprog T): prog (BFILE.memstate * (T * unit)) :=
+  match fp with
+  | FBasic p => fbasic_to_prog mscs p
+  | FBind p bp => x <- (fprog_to_prog mscs p);; (fbasic_to_prog (fst x) (bp (fst (snd x))))
+  end.
+
+Definition permission_secure_fbasic {T} d bm hm mscs pr (p: fbasic T) :=
+  forall tr tr' r mscs' ,
+    exec_fbasic pr tr d bm hm mscs p r mscs' (tr'++tr) ->
+    trace_secure pr tr'.
+
+Definition permission_secure_fprog {T} d bm hm mscs pr (p: fprog T) :=
+  forall tr tr' r mscs' ,
+    fexec pr tr d bm hm mscs p r mscs' (tr'++tr) ->
+    trace_secure pr tr'.
+
+Theorem ps_fbasic2prog:
+  forall T (fp: fbasic T) d bm hm mscs pr,
+    permission_secure d bm hm pr (fbasic_to_prog mscs fp) ->
+    permission_secure_fbasic d bm hm mscs pr fp.
+Proof.
+  unfold permission_secure_fbasic, permission_secure; intros.
+  inversion H0; subst; sigT_eq; clear H0; eauto.
+Qed.
+
+Theorem ps_fbasic2fprog:
+  forall T (fp: fbasic T) d bm hm mscs pr,
+    permission_secure_fbasic d bm hm mscs pr fp ->
+    permission_secure_fprog d bm hm mscs pr (FBasic fp).
+Proof.
+  unfold permission_secure_fbasic, permission_secure_fprog; intros.
+  inversion H0; subst; sigT_eq; clear H0; eauto.
+Qed.
+
+Lemma trace_app_fbasic:
+  forall T (fp: fbasic T) tr d bm hm mscs pr out mscs' tr',
+    exec_fbasic pr tr d bm hm mscs fp out mscs' tr' ->
+    exists tr'', tr' = tr''++tr.
+Proof.
+  intros;
+  inversion H; subst; sigT_eq;
+  denote exec as Hx; apply trace_app in Hx; auto.
+Qed.
+
+Lemma trace_app_fprog:
+  forall T (fp: fprog T) tr d bm hm mscs pr out mscs' tr',
+    fexec pr tr d bm hm mscs fp out mscs' tr' ->
+    exists tr'', tr' = tr''++tr.
+Proof.
+  induction fp; intros.
+  inversion H; subst; repeat sigT_eq;
+  denote exec_fbasic as Hx; apply trace_app_fbasic in Hx; auto.
+  inversion H; subst; repeat sigT_eq.
+  specialize IHfp with (1:= H13).
+  denote exec_fbasic as Hx; apply trace_app_fbasic in Hx; auto.
+  cleanup; eexists; rewrite app_assoc; eauto.
+  specialize IHfp with (1:= H13); auto.
+Qed.
+  
+Theorem ps_fprog_bind:
+  forall T T' (p: fprog T) (fp: T -> fbasic T') d bm hm mscs pr,
+    permission_secure_fprog d bm hm mscs pr p ->
+    (forall tr d' bm' hm' r mscs' tr',
+       fexec pr tr d bm hm mscs p (Finished d' bm' hm' r) mscs' tr' ->
+       permission_secure_fbasic d' bm' hm' mscs' pr (fp r)) ->
+    permission_secure_fprog d bm hm mscs pr (FBind p fp).
+Proof.
+  unfold permission_secure_fbasic, permission_secure_fprog; intros.
+  inversion H1; subst; repeat sigT_eq; clear H1; eauto.
+  specialize H0 with (1:= H15).
+  apply trace_app_fprog in H15 as Hx; cleanup.
+  apply trace_app_fbasic in H16 as Hx; cleanup.
+  specialize H with (1:=H15).
+  rewrite <- app_assoc in H16; specialize H0 with (1:=H16).
+  apply trace_secure_app; eauto.  
+Qed.
+
+
+(**
+Theorem ps_fprog2prog:
+  forall T (fp: fprog T) d bm hm mscs pr,
+    permission_secure d bm hm pr (fprog_to_prog mscs fp) ->
+    permission_secure_fprog d bm hm mscs pr fp.
+Proof.
+  induction fp; intros.
+  apply ps_fbasic2fprog.
+  simpl in H.
+  apply ps_fbasic2prog; auto.
+  simpl in H.
+  unfold permission_secure_fprog, permission_secure in *; intros.
+
+  inversion H0; subst; repeat sigT_eq; clear H0; eauto.
+Abort.
+
+(* this direction requires crashes *)
+Theorem ps_prog2fb:
+  forall T (fp: fbasic T) d bm hm mscs pr,
+    permission_secure_fbasic d bm hm mscs pr fp ->
+    permission_secure d bm hm pr (fbasic_to_prog mscs fp).
+    
+Proof.
+  unfold permission_secure_fbasic, permission_secure; intros.
+  destruct fp; simpl in *; eapply H; econstructor; eauto.
+Qed.
+*)
+
+
+Theorem permission_secure_fbasic_equivalent:
+  forall T (p: fbasic T) tag Fr Fm Ftop ds sm tree1 tree2 mscs fsxp ilist frees pr d1 bm hm d2,
+    (Fr *
+     LOG.rep (FSXPLog fsxp) (SB.rep fsxp) (LOG.NoTxn ds) (MSLL mscs) sm bm hm *
+     [[[ ds!! ::: (Fm * rep fsxp Ftop tree1 ilist frees mscs sm)]]])%pred d1 ->
+    (Fr *
+     LOG.rep (FSXPLog fsxp) (SB.rep fsxp) (LOG.NoTxn ds) (MSLL mscs) sm bm hm *
+     [[[ ds!! ::: (Fm * rep fsxp Ftop tree2 ilist frees mscs sm)]]])%pred d2 ->
+    permission_secure_fbasic d1 bm hm mscs pr p ->
+    can_access pr tag ->
+    tag <> Public ->
+    equivalent_for tag tree1 tree2 ->
+    permission_secure_fbasic d2 bm hm mscs pr p.
+Proof.
+  intros.
+  apply ps_fbasic2prog.
+Abort.
+
+
+Lemma equivalent_update_nt:
+  forall pathname tree tag f1 f2 inum,
+    tag <> (DFOwner f1) ->
+    (DFOwner f1) = (DFOwner f2) ->
+    tree_names_distinct tree ->
+    equivalent_for tag (update_subtree pathname (TreeFile inum f1) tree)
+                   (update_subtree pathname (TreeFile inum f2) tree).
+Proof.
+  induction pathname; intros.
+  unfold equivalent_for; simpl; intros.
+  destruct (tag_dec tag (DFOwner f1)); try congruence.
+  destruct (tag_dec tag (DFOwner f2)); try congruence.
+  destruct tree.
+  unfold equivalent_for in *; simpl; auto.
+  
+  replace (a::pathname) with ([a]++pathname) by (simpl; auto).
+  destruct (find_subtree [a] (TreeDir n l)) eqn:D.
+  repeat erewrite update_subtree_app; eauto.
+  simpl in D; apply find_subtree_helper_in in D as Hx; cleanup.
+  simpl.
+  repeat rewrite map_app; simpl.
+  destruct (String.string_dec a a); try congruence.
+  inversion H1; subst.
+  rewrite map_app in H5; simpl in H5;
+  apply NoDup_remove_2 in H5; intuition.
+  repeat rewrite update_subtree_notfound; intuition.
+  unfold equivalent_for in *; simpl; auto.
+  repeat rewrite map_app; simpl.
+  erewrite IHpathname; eauto.
+  rewrite map_app in H4; apply forall_app_l in H4; inversion H4; auto.
+
+  eapply find_subtree_app_none in D.
+  repeat erewrite update_subtree_path_notfound; eauto.
+  unfold equivalent_for in *; simpl; auto.
+Qed.
+
+
+
+
+Lemma map_app_exists:
+  forall A B (l l0 l1: list A) (f: A -> B),
+    map f (l0++l1) = map f l ->
+    exists l0' l1',
+      l = l0'++l1' /\
+      length l0' = length l0 /\
+      length l1' = length l1. 
+Proof.
+  induction l; simpl ; intros.
+  rewrite map_app in H.
+  apply app_eq_nil in H.
+  cleanup.
+  apply map_eq_nil in H; apply map_eq_nil in H0.
+  exists l0, l1.
+  cleanup; eauto.
+  destruct l0; simpl in *.
+  destruct l1;  simpl in *; try congruence.
+  inversion H.
+  assert (map f ([]++l1) = map f l). simpl; auto.
+  specialize IHl with (1:=H0).
+  cleanup.
+  apply length_zero_iff_nil in H4; cleanup.
+  exists nil, (a::x0).
+  simpl; eauto.
+  
+  inversion H.
+  specialize IHl with (1:=H2).
+  cleanup.
+  exists (a::x), (x0).
+  simpl; eauto.
+Qed.
+
+Lemma app_inv_length:
+  forall A (l1 l2 l3 l4: list A),
+    length l1 = length l2 ->
+    l1 ++ l3 = l2 ++ l4 ->
+    l1 = l2 /\ l3 = l4.
+Proof.
+  induction l1; intros;
+  destruct l2; simpl in *; try congruence.
+  eauto.
+  inversion H; inversion H0; subst.
+  apply IHl1 in H4; destruct H4; subst; eauto.
+Qed.
+
+Lemma equivalent_for_find_subtree:
+  forall pathname tree1 tree2 t inum f,
+    equivalent_for t tree1 tree2 ->
+    find_subtree pathname tree1 = Some (TreeFile inum f) ->
+    DFOwner f = t ->
+    tree_names_distinct tree1 ->
+    tree_names_distinct tree2 ->
+    find_subtree pathname tree2 = Some (TreeFile inum f).
+Proof.
+  induction pathname; intros.
+  {
+    simpl in *.
+    unfold equivalent_for, filter in *.
+    destruct f; simpl in *.
+    cleanup; simpl in *.
+    destruct (tag_dec t t); try congruence.
+    
+    destruct tree2; simpl in *; intuition.
+    destruct d; simpl in *.
+    destruct (tag_dec t DFOwner).
+    cleanup; auto.
+    inversion H; subst; intuition.
+    inversion H.
+  }
+  {
+    destruct tree1; try solve [ simpl in *; congruence].
+    destruct tree2; try solve [ simpl in *; congruence].
+    {
+      simpl in *.
+      unfold equivalent_for, filter in H.
+      destruct (tag_dec t (DFOwner d)); try congruence.
+    }
+    {
+      unfold equivalent_for in *.
+      eapply lookup_firstelem_path in H0.
+      cleanup.
+      simpl in H0.
+      apply find_subtree_helper_in in H0 as Hx; cleanup.
+      specialize IHpathname with (2:=H4).
+      inversion H; subst; clear H.
+      eapply map_app_exists in H6 as Hx; cleanup.
+      destruct x3.
+      simpl in H5.
+      inversion H5.
+      destruct p.
+      repeat rewrite map_app in H6.
+      apply app_inv_length in H6; [|repeat rewrite map_length; auto]; cleanup.
+      simpl in H6.
+      inversion H6; subst.
+      eapply IHpathname in H9; eauto.
+      replace (s::pathname) with ([s]++pathname) by (simpl; auto).
+      erewrite <- find_subtree_extend; eauto.
+      apply find_subtree_leaf_in.
+      intuition.
+      eapply tree_names_distinct_nodup; eauto.
+      inversion H2.
+      rewrite map_app in H11.
+      eapply forall_app_l in H11.
+      simpl in H11; inversion H11; auto.
+      inversion H3.
+      rewrite map_app in H11.
+      eapply forall_app_l in H11.
+      simpl in H11; inversion H11; auto.
+    }
+  }
+Qed.
+
+(** Security Examples **)
+
+Theorem write_same_except_after:
+  forall Fr Fm Fd Ftop ds sm pathname f tree vs mscs mscs1 fsxp ilist frees pr off v1 inum tr d bm hm d1 bm1 hm1 tr1 (r1: res unit),
+  exec_fbasic pr tr d bm hm mscs (FWrite fsxp inum off v1) (Finished d1 bm1 hm1 r1) mscs1 tr1 ->
+  (Fr * [[ sync_invariant Fr ]] *
+     LOG.rep (FSXPLog fsxp) (SB.rep fsxp) (LOG.NoTxn ds) (MSLL mscs) sm bm hm *
+      [[[ ds!! ::: (Fm * rep fsxp Ftop tree ilist frees mscs sm)]]] *
+      [[ find_subtree pathname tree = Some (TreeFile inum f) ]] *
+      [[[ (DFData f) ::: (Fd * off |-> vs) ]]])%pred d ->
+   exists tree1 fsxp1 ds1 sm1 ilist1 frees1,
+    (Fr *
+     LOG.rep (FSXPLog fsxp1) (SB.rep fsxp1) (LOG.NoTxn ds1) (MSLL mscs1) sm1 bm1 hm1 *
+      [[[ ds1!! ::: (Fm * rep fsxp1 Ftop tree1 ilist1 frees1 mscs1 sm1)]]])%pred d1 /\
+    same_except (DFOwner f) tree tree1.
+Proof.
+  intros.
+  inversion H; subst; sigT_eq; clear H.
+  pose proof (write_post _ H0 H17) as Hspec1.
+  apply sep_star_or_distr in Hspec1.
+  apply pimpl_or_apply in Hspec1.
+  intuition; destruct_lift H;
+  do 6 eexists;
+  split; [pred_apply; cancel; eauto | |pred_apply; cancel; eauto |].
+  unfold same_except, equivalent_for; eauto.
+  destruct_lift H0.
+  erewrite <- update_subtree_same at 1; eauto.
+  unfold same_except; intros.
+  eapply equivalent_update_nt; cleanup; eauto.
+  destruct_lift H1; eapply rep_tree_names_distinct; eauto.
+  destruct_lift H1; eapply rep_tree_names_distinct; eauto.
+Qed.
+
+
+Theorem write_same_except_two:
+  forall Fr Fm Fd Ftop ds sm pathname f tree vs mscs mscs1 mscs2 fsxp ilist frees pr off v1 v2 inum tr d bm hm d1 bm1 hm1 d2 bm2 hm2 tr1 (r1 r2: res unit) tr2,
+  exec_fbasic pr tr d bm hm mscs (FWrite fsxp inum off v1) (Finished d1 bm1 hm1 r1) mscs1 tr1 ->
+  exec_fbasic pr tr d bm hm mscs (FWrite fsxp inum off v2) (Finished d2 bm2 hm2 r2) mscs2 tr2 ->
+  (Fr * [[ sync_invariant Fr ]] *
+     LOG.rep (FSXPLog fsxp) (SB.rep fsxp) (LOG.NoTxn ds) (MSLL mscs) sm bm hm *
+      [[[ ds!! ::: (Fm * rep fsxp Ftop tree ilist frees mscs sm)]]] *
+      [[ find_subtree pathname tree = Some (TreeFile inum f) ]] *
+      [[[ (DFData f) ::: (Fd * off |-> vs) ]]])%pred d ->
+    exists tree1 fsxp1 ds1 sm1 ilist1 frees1 tree2 fsxp2 ds2 sm2 ilist2 frees2,
+    (Fr *
+     LOG.rep (FSXPLog fsxp1) (SB.rep fsxp1) (LOG.NoTxn ds1) (MSLL mscs1) sm1 bm1 hm1 *
+      [[[ ds1!! ::: (Fm * rep fsxp1 Ftop tree1 ilist1 frees1 mscs1 sm1)]]])%pred d1 /\
+    (Fr *
+     LOG.rep (FSXPLog fsxp2) (SB.rep fsxp2) (LOG.NoTxn ds2) (MSLL mscs2) sm2 bm2 hm2 *
+     [[[ ds2!! ::: (Fm * rep fsxp2 Ftop tree2 ilist2 frees2 mscs2 sm2)]]])%pred d2 /\
+    same_except (DFOwner f) tree1 tree2.
+Proof.
+  intros.
+  inversion H; subst; sigT_eq; clear H.
+  inversion H0; subst; sigT_eq; clear H0.
+  pose proof (write_post _ H1 H18) as Hspec1.
+  pose proof (write_post _ H1 H17) as Hspec2.
+  apply sep_star_or_distr in Hspec1.
+  apply pimpl_or_apply in Hspec1.
+  intuition.
+  destruct_lift H; intuition.
+  apply sep_star_or_distr in Hspec2.
+  apply pimpl_or_apply in Hspec2.
+  intuition.
+  destruct_lift H2; intuition.
+  do 12 eexists.
+  split.
+  clear H12.
+  pred_apply; safecancel.
+  split.
+  pred_apply; cancel; eauto.
+  unfold same_except, equivalent_for; eauto.
+
+  destruct_lift H2; intuition.
+
+  destruct_lift H; intuition.
+  apply sep_star_or_distr in Hspec2.
+  apply pimpl_or_apply in Hspec2.
+  intuition.
+  destruct_lift H2; intuition.
+  destruct_lift H2; intuition.
+  do 12 eexists.
+  split.
+  pred_apply; cancel; eauto.
+  split.
+  pred_apply; cancel; eauto.
+  unfold same_except; intros.
+  eapply equivalent_update_nt; cleanup; eauto.
+  destruct_lift H1; eapply rep_tree_names_distinct; eauto.
+Qed.
+
+
+Lemma read_equivalent_return:
+  forall pathname f pr off vs inum Fd
+    Fr1 Fm1 Ftop1 ds1 sm1 tree1 mscs1 mscs1' fsxp1 ilist1 frees1 d1 bm1 hm1 d1' bm1' hm1' tr1 tr1'
+    Fr2 Fm2 Ftop2 ds2 sm2 tree2 mscs2 mscs2' fsxp2 ilist2 frees2 d2 bm2 hm2 d2' bm2' hm2' tr2 tr2'
+    (r1 r2: block * res unit),
+  exec_fbasic pr tr1 d1 bm1 hm1 mscs1 (FRead fsxp1 inum off) (Finished d1' bm1' hm1' r1) mscs1' tr1' ->
+  exec_fbasic pr tr2 d2 bm2 hm2 mscs2 (FRead fsxp2 inum off) (Finished d2' bm2' hm2' r2) mscs2' tr2' ->
+  (Fr1 * [[ sync_invariant Fr1 ]] *
+     LOG.rep (FSXPLog fsxp1) (SB.rep fsxp1) (LOG.NoTxn ds1) (MSLL mscs1) sm1 bm1 hm1 *
+      [[[ ds1!! ::: (Fm1 * rep fsxp1 Ftop1 tree1 ilist1 frees1 mscs1 sm1)]]] *
+      [[ find_subtree pathname tree1 = Some (TreeFile inum f) ]] *
+      [[[ (DFData f) ::: (Fd * off |-> vs) ]]])%pred d1 ->
+  (Fr2 * [[ sync_invariant Fr2 ]] *
+     LOG.rep (FSXPLog fsxp2) (SB.rep fsxp2) (LOG.NoTxn ds2) (MSLL mscs2) sm2 bm2 hm2 *
+     [[[ ds2!! ::: (Fm2 * rep fsxp2 Ftop2 tree2 ilist2 frees2 mscs2 sm2)]]])%pred d2 ->
+  equivalent_for (DFOwner f) tree1 tree2 ->
+  r1 = r2.
+Proof.  
+  intros.
+  assert (A: (Fr2 * [[ sync_invariant Fr2 ]] *
+     LOG.rep (FSXPLog fsxp2) (SB.rep fsxp2) (LOG.NoTxn ds2) (MSLL mscs2) sm2 bm2 hm2 *
+      [[[ ds2!! ::: (Fm2 * rep fsxp2 Ftop2 tree2 ilist2 frees2 mscs2 sm2)]]] *
+      [[ find_subtree pathname tree2 = Some (TreeFile inum f) ]] *
+      [[[ (DFData f) ::: (Fd * off |-> vs) ]]])%pred d2).
+  destruct_lift H1; pred_apply; cancel.
+  apply rep_tree_names_distinct in H4.
+  apply rep_tree_names_distinct in H5.
+  eapply equivalent_for_find_subtree; eauto.
+  inversion H; subst; sigT_eq; clear H.
+  inversion H0; subst; sigT_eq; clear H0.
+  pose proof (read_post _ H1 H19) as Hspec1.
+  pose proof (read_post _ A H18) as Hspec2.
+  destruct_lift Hspec1.
+  repeat rewrite sep_star_or_distr in Hspec1.
+  apply sep_star_or_distr in Hspec1.
+  apply pimpl_or_apply in Hspec1.
+  intuition.
+  destruct_lift H; intuition.
+  repeat rewrite sep_star_or_distr in Hspec2.
+  apply sep_star_or_distr in Hspec2.
+  apply pimpl_or_apply in Hspec2.
+  intuition.
+  destruct_lift H0; intuition.
+  admit. (* isError hides the error so can't show equality *) 
+  destruct_lift H0; intuition.
+  
+  destruct_lift H; intuition.
+  repeat rewrite sep_star_or_distr in Hspec2.
+  apply sep_star_or_distr in Hspec2.
+  apply pimpl_or_apply in Hspec2.
+  intuition.
+  destruct_lift H0; intuition.
+  destruct_lift H0; intuition.
+Admitted.
+
+
+
+
+
+
+
+
+
+
+
+
+
+
+
+
+
+
+
+
+
+
+
+
+
+
+
+
+
+
+
+
+
+
+
+
+
+
+
+
+
+
+
+
+
+
+
+
+
+
+
+
+(** this axioms may simplify tree equivalence after execution proofs *)
+Axiom one_tag_per_user:
+  forall pr t t',
+    t <> Public ->
+    t' <> Public ->
+    can_access pr t ->
+    can_access pr t' ->
+    t = t'.
+
+Axiom one_user_per_tag:
+  forall pr pr' t,
+    t <> Public ->
+    can_access pr t ->
+    can_access pr' t ->
+    pr = pr'.
+
+
+Definition sys_rep Fr Fm Ftop fsxp ds sm tree ilist frees mscs bm hm:=
+  (Fr * [[ sync_invariant Fr ]] *
+   LOG.rep (FSXPLog fsxp) (SB.rep fsxp) (LOG.NoTxn ds) (MSLL mscs) sm bm hm *
+   [[[ ds!! ::: (Fm * rep fsxp Ftop tree ilist frees mscs sm)]]])%pred.
+
+
+
+
+
+Lemma return_indistinguishable:
+forall T (p: fprog T) pr,
+
+(forall tag, can_access pr tag ->  equivalent_for tag tree1 tree2) ->
+sys_rep Fr1 Fm1 Ftop1 fsxp1 ds1 sm1 tree1 ilist1 frees1 mscs1 bm1 hm1 d1 ->
+sys_rep Fr2 Fm2 Ftop2 fsxp2 ds2 sm2 tree2 ilist2 frees2 mscs2 bm2 hm2 d2 ->
+(** this represents the residual part of the precondition.
+  e.g. a file existing and file having a block in the given offset etc. **)
+satisfies_precondition tree1 p ->
+satisfies precondition tree2 p ->
+fexec pr tr1 d1 bm1 hm1 mscs1 p (RFinished d1' bm1' hm1' r1) mscs1' tr1' ->
+fexec pr tr2 d2 bm2 hm2 mscs2 p (RFinished d2' bm2' hm2' r2) mscs2' tr2' ->
+  
+r1 = r2.
+
+
+
+
+
+  
+
+(** This is an alternative, stronger lemma which requires 
+    proving an existence of a successful execution from equivalent tree. 
+    I am not sure this version is provable in our framnework. **)
+Lemma return_indistinguishable_alternative:
+forall T (p: fprog T) pr,
+    
+(forall tag, can_access pr tag ->  equivalent_for tag tree1 tree2) ->
+sys_rep Fr1 Fm1 Ftop1 fsxp1 ds1 sm1 tree1 ilist1 frees1 mscs1 bm1 hm1 d1 ->
+sys_rep Fr2 Fm2 Ftop2 fsxp2 ds2 sm2 tree2 ilist2 frees2 mscs2 bm2 hm2 d2 ->
+satisfies_precondition tree1 p ->
+satisfies precondition tree2 p ->
+fexec pr tr1 d1 bm1 hm1 mscs1 p (RFinished d1' bm1' hm1' r1) mscs1' tr1' ->
+  
+exists d2' bm2' hm2' r2 mscs2' tr2',
+fexec pr tr2 d2 bm2 hm2 mscs2 p (RFinished d2' bm2' hm2' r2) mscs2' tr2' /\
+r1 = r2.
+
+
+
+  
+
+  
+(** This lemma proves that -combined with two_exec_return_indistinguishable- 
+   interleaving syscalls from different users will preserve isolation.
+   it inforamlly states the parts that user pr can't reach will stay equivalent 
+   after series of syscalls from that user. **)
+Lemma no_effect_on_others: forall T (p: fprog T) pr tag,
+
+~can_access pr tag ->
+equivalent_for tag tree1 tree2 ->
+
+sys_rep Fr1 Fm1 Ftop1 fsxp1 ds1 sm1 tree1 ilist1 frees1 mscs1 bm1 hm1 d1 ->
+sys_rep Fr2 Fm2 Ftop2 fsxp2 ds2 sm2 tree2 ilist2 frees2 mscs2 bm2 hm2 d2 ->
+satisfies_precondition tree1 p ->
+satisfies precondition tree2 p ->
+fexec pr tr1 d1 bm1 hm1 mscs1 p (RFinished d1' bm1' hm1' r1) mscs1' tr1' ->
+fexec pr tr2 d2 bm2 hm2 mscs2 p (RFinished d2' bm2' hm2' r2) mscs2' tr2' ->
+    
+exists ds1' sm1' tree1' ilist1' frees1' ds2' sm2' tree2' ilist2' frees2',
+sys_rep Fr1 Fm1 Ftop1 fsxp1 ds1' sm1' tree1' ilist1' frees1' mscs1' bm1' hm1' d1' /\
+sys_rep Fr2 Fm2 Ftop2 fsxp2 ds2' sm2' tree2' ilist2' frees2' mscs2' bm2' hm2' d2' /\
+equivalent_for tag tree1' tree2'.
+
+
+    
+
+
+
+(** This version is not provable due to directories being public. 
+    Any syscall that changes the directory structure violates this theorem *)
+Lemma no_effect_on_others_alternative:
+forall T (p: fprog T) pr,
+sys_rep Fr Fm Ftop fsxp ds sm tree ilist frees mscs bm hm d ->
+satisfies_precondition tree p ->
+fexec pr tr d bm hm mscs p (RFinished d' bm' hm' r') mscs' tr' -> 
+
+exists ds1' sm1' tree1' ilist1' frees1',
+  sys_rep Fr Fm Ftop fsxp' ds' sm' tree' ilist' frees' mscs' bm' hm' d' /\
+  (forall tag, ~can_access pr tag -> equivalent_for tag tree1 tree1').
+
+
+
+
+
+
+
+(** Another unprovable theorem due to public files / directories. *)
+Lemma independent_from_other_users:
+forall T T' (p: fprog T) (p': fprog T') pr pr',
+
+sys_rep Fr Fm Ftop fsxp ds sm tree ilist frees mscs bm hm d ->
+satisfies_precondition tree p ->
+fexec pr tr d bm hm mscs p (RFinished d' bm' hm' r') mscs' tr' ->
+sys_rep Fr Fm Ftop fsxp' ds' sm' tree' ilist' frees' mscs' bm' hm' d' ->
+
+satisfies_precondition tree p ->
+satisfies_precondition tree' p' ->
+fexec pr' tr d bm hm mscs p' (RFinished d1' bm1' hm1' r1') mscs1' tr1' ->
+fexec pr' tr' d' bm' hm' mscs' p' (RFinished d2' bm2' hm2' r2') mscs2' tr2' ->
+
+r1' = r2'.
+
+
+
+
+
+    
+
+    
+(** CRASHES **)
+
+
+(** One shortcoming of the below lemma is that 
+    it starts execution from a synced disc. 
+    This requirement is imposed by the second part of the conclusion.
+    if we would allow from some arbitrary disk, 
+    then it could be recovered to a state 
+    that is even before where p starts to execute.
+    If that is the case, I don't know how to prove 
+    the property second part wants to prove. **)
+Lemma two_exec_recover_equivalent:
+  forall T (p: fprog T) pr,
+
+(forall tag, can_access pr tag ->  equivalent_for tag tree1 tree2) ->
+sys_rep Fr1 Fm1 Ftop1 fsxp1 (ds1,[]) sm1 tree1 ilist1 frees1 mscs1 bm1 hm1 d1 ->
+sys_rep Fr2 Fm2 Ftop2 fsxp2 (ds2,[]) sm2 tree2 ilist2 frees2 mscs2 bm2 hm2 d2 ->
+satisfies_precondition tree1 p ->
+satisfies precondition tree2 p ->
+fexec pr tr1 d1 bm1 hm1 mscs1 p (RRecovered d1' bm1' hm1' r1) mscs1' tr1' ->
+fexec pr tr2 d2 bm2 hm2 mscs2 p (RRecovered d2' bm2' hm2' r2) mscs2' tr2' ->
+
+exists Fr1' Fm1' Ftop1' fsxp1' ds1' sm1' tree1' ilist1' frees1'
+   Fr2' Fm2' Ftop2' fsxp2' ds2' sm2' tree2' ilist2' frees2',
+sys_rep Fr1 Fm1 Ftop1 fsxp1 (ds1', []) sm1'
+        tree1' ilist1' frees1' mscs1' bm1' hm1' d1' /\
+sys_rep Fr2 Fm2 Ftop2 fsxp2 (ds2', []) sm2'
+        tree2' ilist2' frees2' mscs2' bm2' hm2' d2' /\
+equivalent_for tag tree1' tree2' /\
+
+  (** this part says that the disks we recovered are reachable by 
+      executing only a prefix of the program p. This has an implication that 
+      we didn't recover a data to a wrong owner **)
+exists n,
+(exists d1'' bm1'' hm1'' r1' mscs1'' tr1'' ds1'' sm1'' ilist1'' frees1'',
+  fexec pr tr1 d1 bm1 hm1 mscs1 (firstn_steps n p)
+        (RFinished d1'' bm1'' hm1'' r1') mscs1'' tr1'' /\
+  sys_rep Fr1 Fm1 Ftop1 fsxp1 ds1'' sm1''
+          tree1' ilist1'' frees1'' mscs1'' bm1'' hm1'' d1'' /\
+  ds1''!! = ds1') /\
+(exists d2'' bm2'' hm2'' r2' mscs2'' tr2'' ds2'' sm2'' ilist2'' frees2'',
+  fexec pr tr2 d2 bm2 hm2 mscs2 (firstn_steps n p)
+        (RFinished d2'' bm2'' hm2'' r2') mscs2'' tr2'' /\
+  sys_rep Fr2 Fm2 Ftop2 fsxp2 ds2'' sm2''
+          tree2' ilist2'' frees2'' mscs2'' bm2'' hm2'' d2'' /\
+  ds2''!! = ds2!).
